added a big test case

theories/wz_bb.v
@@ -1,6 +1,11 @@
 From Coq Require Import Lia Wf_nat.
 From Coq Require Import List.
+From Coq Require Import BinNat Strings.Byte.
+From Coq Require Import ZArith ZArith.Int ZArith.BinInt ZArith.Zpower.
+From compcert Require Integers.
+From mathcomp Require Import ssrnat.
 From Wasm Require Import datatypes list_extra.
+From Wasm Require Import wz_bubble_sort.
 Import ListNotations.
 
 Definition bb_instr: Type := option basic_instruction.
@@ -31,28 +36,40 @@ Definition empty_bb: bb' := init_bb [].
 
 Fixpoint bb's_of_expr' (acc: bb'*list bb') (i: basic_instruction): bb'*list bb' :=
   let bb's_of_expr'' (e: expr) (acc: bb'*list bb') : bb'*list bb' :=
-    List.fold_left bb's_of_expr' e acc
-  in
+    
+    let (bb, bbs) := List.fold_left bb's_of_expr' e acc in
+      (* did we wind up having a bb at the end?*)
+      match bb_instrs bb with
+      (* no, we're done *)
+      | [] => (bb, bbs)
+      (* yes, add it to the list of bbs*)
+      | _ => (empty_bb, ((init_bb (List.rev (bb_instrs bb))::bbs)))
+      end
+    in
     match i with
-      | BI_block _ e1
-      | BI_loop _ e1 =>
+      | BI_block b e1 =>
           let e1_acc := bb's_of_expr'' e1 (empty_bb, []) in
-            (empty_bb,
+            (fst e1_acc,
               (snd e1_acc) 
-              ++ (init_bb (List.rev (i::(bb_instrs (fst acc))))::(snd acc)))
-      | BI_if _ e1 e2 =>
+              ++ (init_bb (List.rev ((BI_block b [])::(bb_instrs (fst acc))))::(snd acc)))
+      | BI_loop b e1 =>
+          let e1_acc := bb's_of_expr'' e1 (empty_bb, []) in
+            (fst e1_acc,
+              (snd e1_acc) 
+              ++ (init_bb (List.rev ((BI_loop b [])::(bb_instrs (fst acc))))::(snd acc)))
+      | BI_if b e1 e2 =>
           let e2_acc := bb's_of_expr'' e2 (empty_bb, []) in
           let e1_acc := bb's_of_expr'' e1 (empty_bb, []) in
             (empty_bb,
               (snd e2_acc)
               ++ (snd e1_acc) 
-              ++ (init_bb (List.rev (i::(bb_instrs (fst acc))))::(snd acc)))
+              ++ (init_bb (List.rev ((BI_if b [] [])::(bb_instrs (fst acc))))::(snd acc)))
     | BI_unreachable
     | BI_br _
     | BI_br_if _
     | BI_br_table _ _
     | BI_return =>
-        (init_bb [], ((init_bb (List.rev (i::(bb_instrs (fst acc)))))::(snd acc)))
+        (empty_bb, ((init_bb (List.rev (i::(bb_instrs (fst acc)))))::(snd acc)))
     | _ => 
         (init_bb (i::(bb_instrs (fst acc))), (snd acc))
   end.
@@ -63,9 +80,9 @@ Definition bb's_of_expr (e: expr): list bb' :=
     (* did we wind up having a bb at the end?*)
     match bb_instrs bb with
     (* no, we're done *)
-    | [] => bbs
+    | [] => List.rev bbs
     (* yes, add it to the list of bbs*)
-    | _ => List.rev ((init_bb (List.rev (bb_instrs bb))::(List.rev bbs)))
+    | _ => List.rev ((init_bb (List.rev (bb_instrs bb))::bbs))
     end.
 
 (* The simplest basic block *)
@@ -105,6 +122,181 @@ forall v1 v2 v3 l,
              bb_pred := []; bb_succ := [] |}].
 Proof.
   reflexivity.
+Qed.
+
+Definition i32_of n: i32 := Wasm_int.Int32.repr n.
+
+Definition bubble_sort_expr: expr :=
+[
+    BI_block (BT_id 0%num) [
+        BI_local_get 0%num;
+        BI_const_num (VAL_int32 (i32_of 2));
+        BI_relop T_i32 (Relop_i (ROI_lt SX_S));
+        BI_br_if 0%num;
+        BI_local_get 0%num;
+        BI_const_num (VAL_int32 (i32_of (-1)));
+        BI_binop T_i32 (Binop_i BOI_add);
+        BI_local_tee 2%num;
+        BI_local_set 3%num;
+        BI_const_num (VAL_int32 (i32_of 0));
+        BI_local_set 4%num;
+        BI_loop  (BT_id 2%num) [
+            BI_local_get 3%num;
+            BI_local_set 5%num;
+            BI_const_num (VAL_int32 (i32_of 0));
+            BI_local_set 6%num;
+            BI_block (BT_id 0%num) [
+                BI_local_get 4%num;
+                BI_local_tee 7%num;
+                BI_local_get 0%num;
+                BI_binop T_i32 (Binop_i BOI_sub);
+                BI_const_num (VAL_int32 (i32_of (-2)));
+                BI_relop T_i32 (Relop_i (ROI_gt SX_S));
+                BI_br_if 0%num;
+                BI_loop (BT_id 4%num) [
+                    BI_block (BT_id 0%num) [
+                        BI_local_get 1%num;
+                        BI_local_get 6%num;
+                        BI_local_tee 3%num;
+                        BI_const_num (VAL_int32 (i32_of 2));
+                        BI_binop T_i32 (Binop_i BOI_shl);
+                        BI_binop T_i32 (Binop_i BOI_add);
+                        BI_local_tee 6%num;
+                        BI_load T_i32 None {| memarg_offset := 0%num;  memarg_align := 0%num |};
+                        BI_local_tee 4%num;
+                        BI_local_get 1%num;
+                        BI_local_get 3%num;
+                        BI_const_num (VAL_int32 (i32_of 1));
+                        BI_binop T_i32 (Binop_i BOI_add);
+                        BI_local_tee 3%num;
+                        BI_const_num (VAL_int32 (i32_of 2));
+                        BI_binop T_i32 (Binop_i BOI_shl);
+                        BI_binop T_i32 (Binop_i BOI_add);
+                        BI_local_tee 8%num;
+                        BI_load T_i32 None {| memarg_offset := 0%num;  memarg_align := 0%num |};
+                        BI_local_tee 9%num;
+                        BI_relop T_i32 (Relop_i (ROI_le SX_S));
+                        BI_br_if 0%num;
+                        BI_local_get 6%num;
+                        BI_local_get 9%num;
+                        BI_store T_i32 None {| memarg_offset := 0%num;  memarg_align := 0%num |};
+                        BI_local_get 8%num;
+                        BI_local_get 4%num;
+                        BI_store T_i32 None {| memarg_offset := 0%num;  memarg_align := 0%num |}
+                    ];
+                    BI_local_get 3%num;
+                    BI_local_set 6%num;
+                    BI_local_get 3%num;
+                    BI_local_get 5%num;
+                    BI_relop T_i32 (Relop_i ROI_ne);
+                    BI_br_if 0%num
+                ]
+            ]
+        ];
+        BI_local_get 5%num;
+        BI_const_num (VAL_int32 (i32_of (-1)));
+        BI_binop T_i32 (Binop_i BOI_add);
+        BI_local_set 3%num;
+        BI_local_get 7%num;
+        BI_const_num (VAL_int32 (i32_of 1));
+        BI_binop T_i32 (Binop_i BOI_add);
+        BI_local_tee 6%num;
+        BI_local_set 4%num;
+        BI_local_get 6%num;
+        BI_local_get 2%num;
+        BI_relop T_i32 (Relop_i ROI_ne);
+        BI_br_if 0%num
+    ]
+].
+
+Definition bubble_sort_bbs: list bb' :=
+[ init_bb[BI_block (BT_id 0%num) []];
+  init_bb[BI_local_get 0%num;
+          BI_const_num (VAL_int32 (i32_of 2));
+          BI_relop T_i32 (Relop_i (ROI_lt SX_S));
+          BI_br_if 0%num];
+  init_bb[BI_local_get 0%num;
+          BI_const_num (VAL_int32 (i32_of (-1)));
+          BI_binop T_i32 (Binop_i BOI_add);
+          BI_local_tee 2%num;
+          BI_local_set 3%num;
+          BI_const_num (VAL_int32 (i32_of 0));
+          BI_local_set 4%num;
+          BI_loop (BT_id 2%num) []];
+  init_bb[BI_local_get 3%num;
+          BI_local_set 5%num;
+          BI_const_num (VAL_int32 (i32_of 0));
+          BI_local_set 6%num;
+          BI_block (BT_id 0%num) []];
+  init_bb[BI_local_get 4%num;
+          BI_local_tee 7%num;
+          BI_local_get 0%num;
+          BI_binop T_i32 (Binop_i BOI_sub);
+          BI_const_num (VAL_int32 (i32_of (-2)));
+          BI_relop T_i32 (Relop_i (ROI_gt SX_S));
+          BI_br_if 0%num];
+  init_bb[BI_loop (BT_id 4%num) []];
+  init_bb[BI_block (BT_id 0%num) []];
+  init_bb[BI_local_get 1%num;
+          BI_local_get 6%num;
+          BI_local_tee 3%num;
+          BI_const_num (VAL_int32 (i32_of 2));
+          BI_binop T_i32 (Binop_i BOI_shl);
+          BI_binop T_i32 (Binop_i BOI_add);
+          BI_local_tee 6%num;
+          BI_load T_i32 None {| memarg_offset := 0%num;  memarg_align := 0%num |};
+          BI_local_tee 4%num;
+          BI_local_get 1%num;
+          BI_local_get 3%num;
+          BI_const_num (VAL_int32 (i32_of 1));
+          BI_binop T_i32 (Binop_i BOI_add);
+          BI_local_tee 3%num;
+          BI_const_num (VAL_int32 (i32_of 2));
+          BI_binop T_i32 (Binop_i BOI_shl);
+          BI_binop T_i32 (Binop_i BOI_add);
+          BI_local_tee 8%num;
+          BI_load T_i32 None {| memarg_offset := 0%num;  memarg_align := 0%num |};
+          BI_local_tee 9%num;
+          BI_relop T_i32 (Relop_i (ROI_le SX_S));
+          BI_br_if 0%num];
+  init_bb[BI_local_get 6%num;
+          BI_local_get 9%num;
+          BI_store T_i32 None {| memarg_offset := 0%num;  memarg_align := 0%num |};
+          BI_local_get 8%num;
+          BI_local_get 4%num;
+          BI_store T_i32 None {| memarg_offset := 0%num;  memarg_align := 0%num |}];
+  init_bb[BI_local_get 3%num;
+          BI_local_set 6%num;
+          BI_local_get 3%num;
+          BI_local_get 5%num;
+          BI_relop T_i32 (Relop_i ROI_ne);
+          BI_br_if 0%num];
+  init_bb[BI_local_get 5%num;
+          BI_const_num (VAL_int32 (i32_of (-1)));
+          BI_binop T_i32 (Binop_i BOI_add);
+          BI_local_set 3%num;
+          BI_local_get 7%num;
+          BI_const_num (VAL_int32 (i32_of 1));
+          BI_binop T_i32 (Binop_i BOI_add);
+          BI_local_tee 6%num;
+          BI_local_set 4%num;
+          BI_local_get 6%num;
+          BI_local_get 2%num;
+          BI_relop T_i32 (Relop_i ROI_ne);
+          BI_br_if 0%num
+    ]
+].
+
+Compute List.length bubble_sort_bbs.
+Compute List.length (bb's_of_expr bubble_sort_expr).
+Compute List.fold_left (fun a x => a + List.length (bb_instrs x)) bubble_sort_bbs 0.
+Compute List.fold_left (fun a x => a + List.length (bb_instrs x)) (bb's_of_expr bubble_sort_expr) 0.
+Compute List.map (fun x => List.length (bb_instrs x)) bubble_sort_bbs.
+Compute List.map (fun x => List.length (bb_instrs x)) (bb's_of_expr bubble_sort_expr).
+
+Example bubble_sort: bb's_of_expr bubble_sort_expr = bubble_sort_bbs.
+Proof.
+  compute. reflexivity.
 Qed.
 
 Lemma bb_instr_not_block: forall (i: basic_instruction) (b: block_type) (e: expr),
