src/extraction.v
@@ -23,6 +23,7 @@ From Wasm Require Import
   wz_ex
   wz_cp
   wz_ssa
+  wz_bubble_sort
   host
   simd_execute
   extraction_instance
@@ -57,4 +58,5 @@ Extraction "extract"
   run_parse_arg
   Extraction_instance
   bblocks_of_expr
+  bubble_sort_expr
   .
